lib/Buckets/BucketWeights.i.dfy
@@ -4,14 +4,14 @@ include "BucketsLib.i.dfy"
 // Assigning weights to buckets guides the flushing algorithm to decide
 // which child to push messages towards. TODO(thance): help!
 //
-// Proposed restructuring: Weights don't belong at the BucketsLib
-// layer.  They belong at the concrete representation layer, where the
-// byte encoding is known.  The only reason they are at this layer is
-// that we use a function definition of flushing, which means we have
-// to deterministically know which flush we are going to do.  If we
-// use a predicate definition instead, then we can describe the
-// non-deterministic universe of valid flushes and concretize at a
-// lower layer.
+// TODO(jonh&robj) Proposed restructuring: Weights don't belong at the
+// BucketsLib layer.  They belong at the concrete representation
+// layer, where the byte encoding is known.  The only reason they are
+// at this layer is that we use a function definition of flushing,
+// which means we have to deterministically know which flush we are
+// going to do.  If we use a predicate definition instead, then we can
+// describe the non-deterministic universe of valid flushes and
+// concretize at a lower layer.
 
 module BucketWeights {
   import Sets
